clightplus_examples/xorlist/xorlist0.v
@@ -5,7 +5,7 @@ Require Import Any.
 Require Import ClightPlusgen.
 Require Import xorlist.
 
-Definition _xor : option Mod.t := compile prog "xorlist".
+Definition _xor : Errors.res Mod.t := compile prog "xorlist".
 
-Theorem valid_xor: exists xor, _xor = Some xor.
+Theorem valid_xor: exists xor, _xor = Errors.OK xor.
 Proof. eauto. Qed.
